src/LAB2/Tokeneer/Tokeneer_Test.dfy
@@ -1,11 +1,17 @@
 class Tokeneer_Test {
-    method Main() {
+    method Main()
+    {
+        print "hello, Dafny\n";
         var id := 114;
         var enrollmentStn := new EnrollmentStn.Init();
         var token := enrollmentStn.enroll(id, 2);
+        assert token != null;
         var IDStnLow := new IDStn.Init(1);
         var IDStnMedium := new IDStn.Init(2);
         var IDStnHigh := new IDStn.Init(3);
+        assert !IDStnLow.doorOpen;
+        assert IDStnLow.validToken(id, token);
+        assert IDStnLow.validClearance(token);
         IDStnLow.open(id, token);
         assert IDStnLow.doorOpen;
     }
